sandbox/Combinators.v
@@ -1,1 +1,281 @@
-../src/Combinators.v
+(** * Some standard combinators *)
+
+Definition Succ := S%nat.  (* an alias for later *)
+
+Require Import Coq.Program.Basics.
+Require Import Coq.Setoids.Setoid.
+Require Import Coq.Classes.RelationClasses.
+Require Import Coq.Classes.Morphisms.
+Require Import Coq.Arith.EqNat.
+Require Export InformationOrdering.
+
+(** ** Abstraction *)
+
+(** Simple I,K,S-abstraction *)
+
+Fixpoint code_abs0 {Var Var' : Set} (b : Var -> option Var') (x : Code Var) :
+  Code Var' :=
+  match x with
+  | code_var v =>
+      match b v with
+      | None => I
+      | Some v' => K * (code_var v')
+      end
+  | l * r => S * code_abs0 b l * code_abs0 b r
+  | TOP => K * TOP
+  | BOT => K * BOT
+  | J => K * J
+  | R => K * R
+  | I => K * I
+  | K => K * K
+  | B => K * B
+  | C => K * C
+  | S => K * S
+  end.
+
+Section code_eq_abs0_sub.
+  Variable Var Var' : Set.
+  Variable b : Var -> option Var'.
+  Variable x : Code Var.
+  Variable y : Code Var'.
+  Let f v := match b v with None => y | Some v' => code_var v' end.
+
+  Lemma code_eq_abs0_sub : code_abs0 b x * y == code_sub f x.
+  Proof.
+    induction x; try (unfold f; simpl; auto; fail).
+      unfold f; simpl; destruct (b v); beta_simpl; auto.
+    rewrite code_sub_ap.
+    unfold code_abs0; fold (@code_abs0 Var).
+    rewrite beta_s; auto.
+  Qed.
+End code_eq_abs0_sub.
+
+Instance code_abs0_proper_le (Var Var' : Set) :
+  Proper (eq ==> code_le ==> code_le) (@code_abs0 Var Var').
+Proof.
+  intros b b' bb' x x' xx'.
+  code_le_weaken; intros ys f.
+  induction ys.
+  - assert (TOP @ f = TOP) as TOP_f; [simpl; auto|].
+    simpl; rewrite <- bb'; intro Hc.
+    rewrite ap_top_conv; rewrite ap_top_conv in Hc.
+    rewrite <- TOP_f; rewrite <- TOP_f in Hc.
+    rewrite <- code_sub_ap; rewrite <- code_sub_ap in Hc.
+    rewrite code_eq_abs0_sub; rewrite code_eq_abs0_sub in Hc.
+    rewrite xx' in Hc; assumption.
+  - set (Ha := code_sub_inverse _ f a); destruct Ha as [a' aa'].
+    simpl.
+    repeat rewrite <- aa'.
+    repeat rewrite <- code_sub_ap.
+    repeat rewrite code_eq_abs0_sub.
+    rewrite xx', bb'; firstorder.
+Qed.
+
+Instance code_abs0_proper_eq (Var Var' : Set) :
+  Proper (eq ==> code_eq ==> code_eq) (@code_abs0 Var Var').
+Proof.
+  intros b b' bb' x x' [xx' x'x]; rewrite <- bb'.
+  split; [rewrite xx' | rewrite x'x]; auto.
+Qed.
+
+(** Efficient I,K,B,C,S,eta-abstraction *)
+
+Fixpoint code_abs {Var Var' : Set} (b : Var -> option Var') (x : Code Var) :
+  Code Var' :=
+  match x with
+  | code_var v =>
+      match b v with
+      | None => I
+      | Some v' => K * (code_var v')
+      end
+  | l * r =>
+      match code_abs b l, code_abs b r with
+      | K * l', I => l'
+      | K * l', K * r' => K * (l' * r')
+      | K * l', r' => B * l' * r'
+      | l', K * r' => C * l' * r'
+      | l', r' => S * l' * r'
+      end
+  | TOP => K * TOP
+  | BOT => K * BOT
+  | J => K * J
+  | R => K * R
+  | I => K * I
+  | K => K * K
+  | B => K * B
+  | C => K * C
+  | S => K * S
+  end.
+
+Section code_eq_abs_sub.
+  Variable Var Var' : Set.
+  Variable b : Var -> option Var'.
+  Variable x : Code Var.
+  Variable y : Code Var'.
+  Let f v := match b v with None => y | Some v' => code_var v' end.
+
+  Lemma code_eq_abs_abs0_ext : code_abs b x * y == code_abs0 b x * y.
+  Proof.
+    induction x; unfold f; simpl; auto.
+    rewrite beta_s.
+    rewrite <- IHc1; clear IHc1.
+    rewrite <- IHc2; clear IHc2.
+    destruct (code_abs b c1);
+    destruct (code_abs b c2);
+    try rewrite beta_s; auto;
+    reflexivity || (
+        destruct c3; try rewrite beta_s; beta_simpl; auto; reflexivity || (
+            destruct c5; try rewrite beta_s; beta_simpl; auto
+    )).
+  Qed.
+
+  Lemma code_eq_abs_sub : code_abs b x * y == code_sub f x.
+  Proof.
+    transitivity (code_abs0 b x * y);
+    [apply code_eq_abs_abs0_ext | apply code_eq_abs0_sub].
+  Qed.
+End code_eq_abs_sub.
+Hint Resolve code_eq_abs_sub.
+
+Lemma code_eq_abs_abs0
+  (Var Var' : Set) (b : Var -> option Var') (x : Code Var) :
+  code_abs b x == code_abs0 b x.
+Proof.
+  eta_expand as y; apply code_eq_abs_abs0_ext.
+Qed.
+
+Instance code_abs_proper_le (Var Var' : Set) :
+  Proper (eq ==> code_le ==> code_le) (@code_abs Var Var').
+Proof.
+  intros b b' bb' x x' xx'.
+  repeat rewrite code_eq_abs_abs0.
+  rewrite bb', xx'; auto.
+Qed.
+
+Instance code_abs_proper_eq (Var Var' : Set) :
+  Proper (eq ==> code_eq ==> code_eq) (@code_abs Var Var').
+Proof.
+  intros b b' bb' x x' xx'.
+  repeat rewrite code_eq_abs_abs0.
+  rewrite bb', xx'; auto.
+Qed.
+
+(** ** Informal lambda notation *)
+
+Definition make_var (Var : Set) (n : nat) : Code (nat + Var) :=
+  code_var (@inl nat Var n).
+
+Definition open_var {Var : Set} (x : Code Var) : Code (nat + Var) :=
+  code_sub (fun v => code_var (inr v)) x.
+
+Definition close_var {Var : Set} (x : Code (nat + Var)) : Code Var :=
+  code_sub (fun v => match v with inr v' => code_var v' | _ => code_top end) x.
+
+Lemma close_open (Var : Set) (x : Code Var) : close_var (open_var x) = x.
+Proof.
+  unfold close_var, open_var.
+  induction x; simpl; auto.
+  rewrite IHx1; rewrite IHx2; auto.
+Qed.
+
+Definition code_lambda {Var : Set} (x y : Code (nat + Var)) :
+  Code (nat + Var) :=
+  let beq_var (v1 v2 : nat + Var) : bool :=
+    match v1, v2 with
+    | inl n1, inl n2 => beq_nat n1 n2
+    | _, _ => false
+    end
+  in
+  match x with
+  | code_var v => code_abs (fun v' => if beq_var v v' then None else Some v') y
+  | _ => BOT  (* TODO implement pattern matching here *)
+  end.
+
+Notation "\ x , y" := (code_lambda x y) : code_scope.
+
+(** ** Standard combinators *)
+
+Section Y.
+  Context {Var : Set}.
+  Let f := make_var Var 0.
+  Let x := make_var Var 1.
+  Definition Y := Eval compute in close_var
+    (\f, (\x, f * (x * x)) * (\x, f * (x * x))).
+    (* ((\x, \f, f * (x * x * f)) * (\x, \f, f * (x * x * f))). *)
+End Y.
+
+Lemma code_eq_y (Var : Set) (f : Code Var) : Y * f == f * (Y * f).
+Proof.
+  unfold Y.
+  rewrite beta_s at 1.
+  rewrite beta_c at 1.
+  rewrite beta_b at 1.
+  rewrite beta_s at 1.
+  rewrite beta_i.
+  rewrite <- beta_s at 1.
+  reflexivity.
+Qed.
+
+Section V.
+  Context {Var : Set}.
+  Let a := make_var Var 0.
+  Let x := make_var Var 1.
+  Definition V := Eval compute in close_var (\a, Y * \x, I || a o x).
+End V.
+
+Lemma code_eq_v (Var : Set) (a : Code Var) : V * a == I || a o (V * a).
+Proof.
+  unfold V at 1; fold (@Y Var).
+  rewrite beta_b at 1.
+  rewrite code_eq_y.
+  rewrite <- (beta_right beta_b) at 1.
+  unfold Y; fold (@V Var).
+  beta_simpl; reflexivity.
+Qed.
+
+Lemma code_eq_v' (Var : Set) (a : Code Var) : V * a == I || (V * a) o a.
+Proof.
+Admitted.
+
+(* The [div] combinator is useful in convergence testing *)
+
+Definition div {Var : Set} : Code Var := Eval compute in V * (C * I * TOP).
+
+Lemma code_eq_div (Var : Set) (x : Code Var) : div * x == x || div * x * TOP.
+Proof.
+  unfold div; fold (@V Var).
+  rewrite code_eq_v at 1; beta_simpl; auto.
+Qed.
+
+Lemma code_eq_div' (Var : Set) (x : Code Var) :
+  div * x == x || div * (x * TOP).
+Proof.
+  unfold div; fold (@V Var).
+  rewrite code_eq_v' at 1; beta_simpl; auto.
+Qed.
+
+Lemma conv_div (Var : Set) (x : Code Var) : conv x <-> conv (div * x).
+Proof.
+  split; intro Hc.
+    rewrite code_eq_div.
+    rewrite pi_j_left.
+    auto.
+  admit. (* TODO use limit characterization of div and induction on probe *)
+Qed.
+
+Lemma conv_div_top (x : Code Empty_set) : conv x <-> div * x == TOP.
+Proof.
+  split.
+    (* OLD
+    intro H; induction H; split; auto; intros Var' c f Hc.
+      rewrite H; rewrite code_eq_div; rewrite pi_j_left; auto.
+    rewrite code_eq_div'; rewrite pi_j_right; rewrite IHconv; auto.
+    *)
+    admit.
+  intros [H' H]; clear H'; unfold code_le in H.
+  (* rewrite <- var_monad_unit_right; rewrite <- beta_i. *)
+  assert (conv (I * (TOP @ code_var) : Code Empty_set)) as Ht; code_simpl; auto.
+  set (Hd := H Empty_set I code_var Ht).
+  code_simpl in Hd.
+  apply conv_div; auto.
+Qed.
