src/Applications.v
@@ -1,4 +1,0 @@
-(** * Applications *)
-
-Require Import Types.
-Open Scope code_scope.
