README.md
@@ -1,16 +1,10 @@
 [![Build Status](https://travis-ci.org/fritzo/hstar.svg?branch=master)](https://travis-ci.org/fritzo/hstar)
-![Proof Status](https://img.shields.io/badge/proofs-44_holes-red.svg?style=flat)
+![Proof Status](https://img.shields.io/badge/proofs-25_holes-red.svg?style=flat)
 
  Holes | File
  -----:|:----------------------------------------------------------------------
-    10 | [Types](src/Types.v)
-     9 | [TypeConstructor](src/TypeConstructor.v)
-     8 | [LeastFixedPoint](src/LeastFixedPoint.v)
-     5 | [BohmTrees](src/BohmTrees.v)
-     4 | [Codes](src/Codes.v)
-     3 | [Combinators](src/Combinators.v)
-     3 | [InformationOrdering](src/InformationOrdering.v)
-     2 | [Nontermination](src/Nontermination.v)
+    21 | [NormalForms](src/NormalForms.v)
+     4 | [Terms](src/Terms.v)
 
 # Inadvertently typed &lambda;-join-calculus
 
